theories/counter_spec_modular.v
@@ -1,0 +1,68 @@
+From iris.algebra Require Import frac.
+From iris.base_logic.lib Require Import invariants.
+From iris.bi.lib Require Import fractional.
+From iris.heap_lang Require Import proofmode notation.
+From iris.prelude Require Import options.
+
+Class modular_counter (Σ : gFunctors) `{!heapGS Σ} := ModularCounter {
+  modular_new_counter : val;
+  modular_incr : val;
+  modular_read : val;
+
+  modular_counter_name : Type;
+  modular_counter_namespace : namespace;
+
+  modular_is_counter : modular_counter_name → val → iProp Σ;
+  modular_handle : modular_counter_name → val → iProp Σ;
+  counter_model : modular_counter_name → Qp → nat → iProp Σ;
+
+  modular_is_counter_persistent γ c ::
+    Persistent (modular_is_counter γ c);
+
+  modular_handle_persistent γ h ::
+    Persistent (modular_handle γ h);
+
+  counter_model_fractional γ n ::
+    Fractional (λ q, counter_model γ q n);
+
+  modular_new_counter_spec (E : coPset) (T : nat) :
+    ↑modular_counter_namespace ⊆ E →
+    {{{ ⌜0 < T⌝ }}}
+      modular_new_counter #T @ E
+    {{{ c γ, RET c;
+        modular_is_counter γ c ∗
+        ([∗ list] i ∈ seq 0 T,
+          modular_handle γ #(i : nat)) ∗
+        counter_model γ (1 / 2)%Qp 0 }}};
+
+  modular_incr_spec
+      (E : coPset) γ c h
+      (P : iProp Σ) (Q : nat → iProp Σ) :
+    ↑modular_counter_namespace ⊆ E →
+    (∀ total,
+      □ (counter_model γ (1 / 2)%Qp total ∗ P
+          ={E ∖ ↑modular_counter_namespace}=∗
+         counter_model γ (1 / 2)%Qp (S total) ∗ Q total)) ⊢
+    {{{ modular_is_counter γ c ∗
+        modular_handle γ h ∗ P }}}
+      modular_incr c h @ E
+    {{{ RET #();
+        modular_is_counter γ c ∗
+        modular_handle γ h ∗
+        ∃ total, Q total }}};
+
+
+  modular_read_spec
+      (E : coPset) γ c
+      (P : iProp Σ) (Q : nat → iProp Σ) :
+    ↑modular_counter_namespace ⊆ E →
+    (∀ total,
+      □ (counter_model γ (1 / 2)%Qp total ∗ P
+          ={E ∖ ↑modular_counter_namespace}=∗
+         counter_model γ (1 / 2)%Qp total ∗ Q total)) ⊢
+    {{{ modular_is_counter γ c ∗ P }}}
+      modular_read c @ E
+    {{{ (total : nat), RET #total;
+        modular_is_counter γ c ∗
+        Q total }}};
+}.
