theories/sharded_counter_modular.v
@@ -1,0 +1,247 @@
+From iris.algebra Require Import agree frac.
+From iris.base_logic.lib Require Import invariants.
+From iris.bi.lib Require Import fractional.
+From iris.heap_lang Require Import proofmode notation.
+From iris.prelude Require Import options.
+
+From summer_project Require Import counter_spec_modular.
+
+
+Definition msc_new_counter : val :=
+  λ: "T", (AllocN "T" #0, "T").
+
+Definition msc_incr : val :=
+  λ: "c" "k",
+    let: "l" := (Fst "c") +ₗ "k" in
+    FAA "l" #1;;
+    #().
+
+Definition msc_sum_loop : val :=
+  rec: "sum" "a" "T" "i" "acc" :=
+    if: "i" = "T" then "acc"
+    else
+      let: "n" := ! ("a" +ₗ "i") in
+      "sum" "a" "T" ("i" + #1) ("acc" + "n").
+
+Definition msc_read : val :=
+  λ: "c",
+    let: "a" := Fst "c" in
+    let: "T" := Snd "c" in
+    msc_sum_loop "a" "T" #0 #0.
+
+Definition msc_modelR : cmra := prodR fracR (agreeR natO).
+
+Class mscG Σ := MSCG {
+  msc_modelG :: inG Σ msc_modelR;
+}.
+
+Definition mscΣ : gFunctors := #[GFunctor msc_modelR].
+
+Global Instance subG_mscΣ Σ : subG mscΣ Σ → mscG Σ.
+Proof. solve_inG. Qed.
+
+Definition mscN : namespace := nroot .@ "sharded_counter_modular".
+
+Definition msc_model_elem (q : Qp) (n : nat) : msc_modelR :=
+  (q, to_agree n).
+Typeclasses Opaque msc_model_elem.
+
+Section model.
+  Context `{!mscG Σ}.
+
+  Global Instance msc_model_elem_fractional γ n :
+    Fractional (λ q, own γ (msc_model_elem q n))%I.
+  Proof.
+    intros p q. rewrite /msc_model_elem -own_op.
+    f_equiv. split; first done. by rewrite /= agree_idemp.
+  Qed.
+
+  Global Instance msc_model_elem_as_fractional γ q n :
+    AsFractional (own γ (msc_model_elem q n))
+      (λ q, own γ (msc_model_elem q n))%I q.
+  Proof. split; first done. apply _. Qed.
+End model.
+
+
+Section proof.
+  Context `{!heapGS Σ, !mscG Σ}.
+  Definition msc_name : Type := gname * nat.
+
+  Definition msc_model
+      (γ : msc_name) (q : Qp) (n : nat) : iProp Σ :=
+    own γ.1 (msc_model_elem q n).
+
+  Global Instance msc_model_fractional γ n :
+    Fractional (λ q, msc_model γ q n).
+  Proof. apply _. Qed.
+
+
+  Definition msc_inv (γ : msc_name) (a : loc) : iProp Σ :=
+    ∃ ns : list nat,
+      ⌜length ns = γ.2⌝ ∗
+      msc_model γ (1 / 2)%Qp (sum_list ns) ∗
+      [∗ list] i ↦ n ∈ ns, (a +ₗ i) ↦ #(n : nat).
+
+  Definition msc_is_counter
+      (γ : msc_name) (c : val) : iProp Σ :=
+    ∃ a : loc,
+      ⌜c = (#a, #(γ.2 : nat))%V⌝ ∗
+      inv mscN (msc_inv γ a).
+
+  Global Instance msc_is_counter_persistent γ c :
+    Persistent (msc_is_counter γ c).
+  Proof. apply _. Qed.
+
+  Definition msc_handle (γ : msc_name) (h : val) : iProp Σ :=
+    ∃ i : nat, ⌜h = #(i : nat)⌝ ∗ ⌜i < γ.2⌝.
+
+  Global Instance msc_handle_persistent γ h :
+    Persistent (msc_handle γ h).
+  Proof. apply _. Qed.
+
+
+
+  Lemma msc_make_handles γt T :
+    ⊢ [∗ list] i ∈ seq 0 T, msc_handle (γt, T) #(i : nat).
+  Proof.
+    iApply big_sepL_intro.
+    iIntros "!>" (k i Hlookup).
+    apply lookup_seq in Hlookup as [-> Hk]. simpl.
+    rewrite /msc_handle.
+    iExists k. iPureIntro. split; first done. exact Hk.
+  Qed.
+
+  Lemma msc_sum_list_insert_S ns i n :
+    ns !! i = Some n →
+    sum_list (<[i := S n]> ns) = S (sum_list ns).
+  Proof.
+    revert i. induction ns as [|m ns IH]; intros [|i] Hlookup;
+      simpl in Hlookup |- *; simplify_eq; first lia.
+    rewrite (IH i Hlookup). lia.
+  Qed.
+
+
+
+  Lemma msc_new_counter_spec E (T : nat) :
+    ↑mscN ⊆ E →
+    {{{ ⌜0 < T⌝ }}}
+      msc_new_counter #T @ E
+    {{{ c γ, RET c;
+        msc_is_counter γ c ∗
+        ([∗ list] i ∈ seq 0 T,
+          msc_handle γ #(i : nat)) ∗
+        msc_model γ (1 / 2)%Qp 0 }}}.
+  Proof.
+    iIntros (Hsubset Φ) "%HT HΦ".
+    rewrite /msc_new_counter. wp_lam.
+    wp_alloc a as "Ha"; first lia.
+    iEval (rewrite Nat2Z.id) in "Ha".
+
+    iMod (own_alloc (msc_model_elem 1%Qp 0)) as (γt) "Hmodel";
+      first done.
+    iDestruct "Hmodel" as "[Hinternal Hclient]".
+
+    iAssert ([∗ list] i ↦ n ∈ replicate T (0 : nat),
+        (a +ₗ i) ↦ #(n : nat))%I with "[Ha]" as "Hcells".
+    { rewrite -(big_sepL_fmap (λ n : nat, #(n : nat))
+          (λ i v, (a +ₗ i) ↦ v)%I (replicate T (0 : nat))).
+      rewrite fmap_replicate /array. iFrame. }
+
+    iMod (inv_alloc mscN _ (msc_inv (γt, T) a)
+      with "[Hinternal Hcells]") as "#Hinv".
+    { iNext. iExists (replicate T (0 : nat)).
+      iSplit; first by rewrite length_replicate.
+      rewrite sum_list_replicate Nat.mul_0_r. iFrame. }
+
+    iPoseProof (msc_make_handles γt T) as "Hhandles".
+    wp_pures.
+    iApply ("HΦ" $! (#a, #T)%V (γt, T)).
+    iFrame "Hhandles Hclient".
+    iExists a. iFrame "Hinv". done.
+  Qed.
+
+
+
+  Lemma msc_incr_spec
+      E γ c h (P : iProp Σ) (Q : nat → iProp Σ) :
+    ↑mscN ⊆ E →
+    (∀ total,
+      □ (msc_model γ (1 / 2)%Qp total ∗ P
+          ={E ∖ ↑mscN}=∗
+         msc_model γ (1 / 2)%Qp (S total) ∗ Q total)) ⊢
+    {{{ msc_is_counter γ c ∗ msc_handle γ h ∗ P }}}
+      msc_incr c h @ E
+    {{{ RET #();
+        msc_is_counter γ c ∗ msc_handle γ h ∗
+        ∃ total, Q total }}}.
+  Proof.
+    iIntros (Hsubset) "#HVS".
+    iIntros (Φ) "!# (#Hcounter & #Hhandle & HP) HΦ".
+    iDestruct "Hcounter" as (a ->) "#Hinv".
+    iDestruct "Hhandle" as (i) "[%Hh %Hi]".
+    subst h.
+
+    rewrite /msc_incr. wp_lam. wp_pures.
+    wp_bind (FAA _ _)%E.
+    iInv mscN as (ns) ">(%Hlen & Hmodel & Hcells)" "Hclose".
+
+    have Hi_ns : i < length ns by lia.
+    destruct (lookup_lt_is_Some_2 ns i Hi_ns) as [n Hn].
+    iDestruct (big_sepL_insert_acc _ _ _ _ Hn with "Hcells")
+      as "[Hl Hcells]".
+
+    wp_faa.
+    iMod ("HVS" $! (sum_list ns) with "[$Hmodel $HP]")
+      as "[Hmodel HQ]".
+
+    iEval (rewrite Z.add_1_r -Nat2Z.inj_succ) in "Hl".
+    iDestruct ("Hcells" $! (S n) with "Hl") as "Hcells".
+    iMod ("Hclose" with "[Hmodel Hcells]") as "_".
+    { iNext. iExists (<[i := S n]> ns).
+      iSplit; first by rewrite length_insert.
+      rewrite (msc_sum_list_insert_S _ _ _ Hn). iFrame. }
+
+    iModIntro. wp_pures.
+    iApply "HΦ".
+    iModIntro.
+    iSplit.
+    { iExists a. iFrame "Hinv". done. }
+    iSplit.
+    { iExists i. iPureIntro. split; done. }
+    iExists (sum_list ns). iFrame.
+  Qed.
+
+
+  Lemma msc_read_spec
+      E γ c (P : iProp Σ) (Q : nat → iProp Σ) :
+    ↑mscN ⊆ E →
+    (∀ total,
+      □ (msc_model γ (1 / 2)%Qp total ∗ P
+          ={E ∖ ↑mscN}=∗
+         msc_model γ (1 / 2)%Qp total ∗ Q total)) ⊢
+    {{{ msc_is_counter γ c ∗ P }}}
+      msc_read c @ E
+    {{{ (total : nat), RET #total;
+        msc_is_counter γ c ∗ Q total }}}.
+  Proof.
+  Admitted.
+
+
+  Definition modular_sharded_counter : modular_counter Σ := {|
+    modular_new_counter := msc_new_counter;
+    modular_incr := msc_incr;
+    modular_read := msc_read;
+    modular_counter_name := msc_name;
+    modular_counter_namespace := mscN;
+    modular_is_counter := msc_is_counter;
+    modular_handle := msc_handle;
+    counter_model := msc_model;
+    modular_is_counter_persistent := msc_is_counter_persistent;
+    modular_handle_persistent := msc_handle_persistent;
+    counter_model_fractional := msc_model_fractional;
+    modular_new_counter_spec := msc_new_counter_spec;
+    modular_incr_spec := msc_incr_spec;
+    modular_read_spec := msc_read_spec;
+  |}.
+
+End proof.
